src/tc/tcutil.fs
@@ -877,7 +877,6 @@ let maybe_assume_result_eq_pure_term env (e:exp) (lc:lcomp) : lcomp =
   let refine () = 
       let c = lc.comp() in
       if not (is_pure_effect env lc.eff_name)
-         || (Util.is_constructor lc.res_typ Const.unit_lid)
       then c
       else if Util.is_partial_return c then c
       else match (compress_typ (Util.comp_result c)).n with 
